order-book/verify/Properties/Order/Complete/DoubleSatisfaction.lean
@@ -1,6 +1,7 @@
 import PlutusCore.UPLC
 import CardanoLedgerApi.V3
 import Blaster
+import Properties.Common
 import Properties.Order.Complete.Spec
 import Properties.Order.Complete.Completeness
 
@@ -8,12 +9,14 @@ import Properties.Order.Complete.Completeness
 
 namespace Properties.Order.Complete.DoubleSatisfaction
 
+open Properties.Common (validatorAccepts)
 open Properties.Order.Complete.Spec (noDoubleSatisfaction)
-open Properties.Order.Complete.Completeness (orderAcceptsProp)
+open Properties.Order.Complete.Completeness (orderValidator)
 
 set_option warn.sorry false
 
-theorem no_double_satisfaction : noDoubleSatisfaction orderAcceptsProp
+theorem no_double_satisfaction :
+    noDoubleSatisfaction (validatorAccepts · orderValidator)
     := by blaster
 
 end Properties.Order.Complete.DoubleSatisfaction
