order-book/verify/Properties/Order/MinimalSingle/DoubleSatisfaction.lean
@@ -1,6 +1,7 @@
 import PlutusCore.UPLC
 import CardanoLedgerApi.V3
 import Blaster
+import Properties.Common
 import Properties.Order.Minimal.DoubleSatisfaction
 import Properties.Order.MinimalSingle.Completeness
 
@@ -8,13 +9,14 @@ import Properties.Order.MinimalSingle.Completeness
 
 namespace Properties.Order.MinimalSingle.DoubleSatisfaction
 
+open Properties.Common (validatorAccepts)
 open Properties.Order.Minimal.DoubleSatisfaction (noDoubleSatisfaction)
-open Properties.Order.MinimalSingle.Completeness (orderMinimalSingleAcceptsProp)
+open Properties.Order.MinimalSingle.Completeness (orderMinimalSingleValidator)
 
 set_option warn.sorry false
 
 theorem no_double_satisfaction :
-    noDoubleSatisfaction orderMinimalSingleAcceptsProp
+    noDoubleSatisfaction (validatorAccepts · orderMinimalSingleValidator)
     := by blaster
 
 end Properties.Order.MinimalSingle.DoubleSatisfaction
